src/DEC2/CTestI1.v
@@ -1,0 +1,325 @@
+(*  DEC 2.0 language specification.
+   Paolo Torrini  
+   Universite' de Lille - CRIStAL-CNRS
+*)
+
+Require Import List.
+Require Import Equality.
+Require Import Eqdep.
+Require Import PeanoNat.
+Require Import Omega.
+Require Import Eqdep FunctionalExtensionality Tactics.
+Require Import JMeq.
+Require Import ProofIrrelevance.
+Require Import GenericMinMax.
+Require Import NMaxMin.
+
+Require Import AuxLibI1.
+Require Import TypSpecI1. 
+Require Import ModTypI1. 
+Require Import LangSpecI1. 
+Require Import StaticSemI1.
+Require Import DynamicSemI1.
+Require Import WeakenI1.
+Require Import UniqueTypI1.
+Require Import DerivDynI1.
+Require Import TransPrelimI1.
+Require Import TSoundnessI1.
+Require Import SReducI1.
+Require Import DetermI1.
+Require Import PreReflI1.
+Require Import ReflectI1.
+Require Import PreInterI1.
+Require Import InterprBaseI1.
+Require Import InterpretI1.
+Require Import CHeadAuxI1.
+
+Require Import ModNat1I1.
+
+Add LoadPath "~/lib/CompCert-3.0.1" as compcert. 
+
+Require Import CTransI1.
+Require Import String.
+
+
+(*Add LoadPath "/home/ptorrx/svnRepos/ptorrx-leuven/trunk/docsLille/develL5/CompCert-3.0.1" as compcert. *)
+(*
+Add LoadPath "/home/ptorrx/lib/CompCert-3.0.1/cfrontend" as compcert.cfrontend.
+Add LoadPath "/home/ptorrx/lib/CompCert-3.0.1/common" as compcert.common.
+*)
+
+Require Import BinNat.
+Require Import Integers.
+
+Require VectorDef.
+
+Require Import compcert.common.AST.
+Require Import compcert.cfrontend.Ctypes.
+Require Import compcert.cfrontend.Csyntax.
+
+Import ListNotations.
+Import Integers.
+
+Import Values.
+
+Module CTest (IdT: ModTyp) <: ModTyp.
+
+Module CTestL := CTrans ModNat1.
+Export CTestL.
+
+Definition Id := CTestL.Id.
+Definition IdEqDec := CTestL.IdEqDec.
+Definition IdEq := CTestL.IdEq.
+Definition W := CTestL.W.
+Definition BInit := CTestL.BInit.
+Definition WP := CTestL.WP.
+
+Open Scope type_scope.
+
+
+(************ TEST ******************)
+
+
+Lemma FEnvWT_nil : FEnvWT nil.
+  unfold FEnvWT.
+  intros.
+  inversion H0.
+Defined.
+  
+Lemma noDup_nil : @noDup Id Value nil.
+  unfold noDup.
+  econstructor.
+Defined.  
+
+Definition transTest_nil := TopLevel0 nil nil FEnvWT_nil noDup_nil.
+
+Eval compute in transTest_nil.                                  
+
+(******************************************************************)
+
+Definition exp1 : Exp := (Val (cst Nat (2%nat))).
+
+Lemma ExpTyping_exp1 : ExpTyping nil nil exp1 Nat.
+repeat econstructor.
+Defined.
+
+Lemma allowed_Nat : Allowed Nat.
+repeat econstructor.
+Defined.
+
+Lemma ExtCAgree_nil : ExtCAgree nil nil.
+econstructor.
+Defined.  
+
+Definition test_exp1 := Exp2CC nil nil nil exp1 Nat
+                          ExpTyping_exp1 nil ExtCAgree_nil nil.
+
+Eval compute in test_exp1.
+
+Definition val1 := (Vint
+             {|
+             Int.intval := 1;
+             Int.intrange := Make32.Z_mod_modulus_range' 1 |}).
+
+Definition typ1 := (Tint I32 Unsigned
+                         {| attr_volatile := false; attr_alignas := None |}).
+
+Definition val1a := (Vint
+             {|
+             Int.intval := 2;
+             Int.intrange := Make32.Z_mod_modulus_range' 2 |}).
+
+
+Definition cexp1 := Csyntax.Eval val1 typ1.
+Definition cexp1a := Csyntax.Eval val1a typ1.
+
+Definition cexp2 := Ecomma cexp1 cexp1a typ1.
+                                                                            
+Definition exp2 := (BindN (Val (cst Nat (1%nat)))
+                                      (Val (cst Nat (2%nat)))).
+
+Lemma ExpTyping_exp2 : ExpTyping nil nil exp2 Nat.
+  repeat econstructor.
+Defined.
+
+Definition test_exp2 := Exp2CC nil nil nil exp2 Nat
+                         ExpTyping_exp2 nil ExtCAgree_nil nil.
+
+Eval compute in test_exp2.
+
+Definition exp3 := (BindN (Val (cst Nat (3%nat))) exp2).
+
+Lemma ExpTyping_exp3 : ExpTyping nil nil exp3 Nat.
+  repeat econstructor.
+Defined.
+
+Definition test_exp3 := Exp2CC nil nil nil exp3 Nat
+                         ExpTyping_exp3 nil ExtCAgree_nil nil.
+
+Eval compute in test_exp3.
+
+
+Definition fun1 : Fun := FC nil (cst Nat (0%nat)) exp3.
+
+Lemma FEnvWT_fun1 (x: Id) : FEnvWT ([(x, fun1)]).
+  unfold FEnvWT, FunWT, fun1.
+  intros.
+  destruct f.
+  simpl in *.
+  destruct (ModNat1.IdEqDec x0 x).
+  inversion e0; subst.
+  inversion H0; subst.
+  simpl in *.
+  repeat econstructor.
+  inversion H0.
+Defined.  
+
+
+Definition cv : string -> Id := id.
+
+Lemma FEnvWT_fun1a : FEnvWT ([(cv "x", fun1)]).
+  eapply FEnvWT_fun1.
+Defined.  
+
+Lemma noDup_fun1 (x: Id) : noDup ([(x, fun1)]).
+  unfold noDup.
+  econstructor.
+  auto.
+  econstructor.
+Defined.
+
+Lemma noDup_fun1a : noDup ([(cv "x", fun1)]).
+  eapply noDup_fun1.
+Defined.  
+
+Definition test_fun1 := TopLevel0 nil ([(cv "x", fun1)])
+                                  FEnvWT_fun1a noDup_fun1a.
+
+Eval native_compute in test_fun1.
+
+Definition exp4 := (BindS (cv "y") (Some Nat) exp3
+                                              (Var (cv "y"))).
+
+Lemma ExpTyping_exp4 : ExpTyping nil nil exp4 Nat.
+  repeat econstructor.
+Defined.
+
+Definition test_exp4 := Exp2CC nil nil nil exp4 Nat
+                         ExpTyping_exp4 nil ExtCAgree_nil nil.
+
+Eval compute in test_exp4.
+
+Definition exp5 := (BindS (cv "z") (Some Nat) exp4
+                                              (BindN (Var (cv "z")) exp4)).
+
+Lemma ExpTyping_exp5 : ExpTyping nil nil exp5 Nat.
+  repeat econstructor.
+Defined.
+
+Definition test_exp5 := Exp2CC nil nil nil exp5 Nat
+                         ExpTyping_exp5 nil ExtCAgree_nil nil.
+
+Eval compute in test_exp5.
+
+Definition exp6 := (BindN (Val (cst Nat (1%nat))) (Val (cst Bool (true)))).
+
+Lemma ExpTyping_exp6 : ExpTyping nil nil exp6 Bool.
+  repeat econstructor.
+Defined.
+
+Definition test_exp6 := Exp2CC nil nil nil exp6 Bool
+                         ExpTyping_exp6 nil ExtCAgree_nil nil.
+
+Eval compute in test_exp6.
+
+Definition exp7 := IfThenElse exp6 exp5 exp4.
+
+Lemma ExpTyping_exp7 : ExpTyping nil nil exp7 Nat.
+  repeat econstructor.
+Defined.
+
+Definition test_exp7 := Exp2CC nil nil nil exp7 Nat
+                         ExpTyping_exp7 nil ExtCAgree_nil nil.
+
+Eval compute in test_exp7.
+
+
+Definition fun2 : Fun := FC nil (cst Nat (0%nat))
+                             (Call (cv "f3") (PS [(Val (cst Nat (4%nat)))])).
+
+Definition fun3 : Fun := FC [(cv "x", Nat)] (cst Nat (0%nat))
+                             (Call (cv "f2") (PS [])).
+
+Definition funEnv23 : funEnv := [(cv "f2", fun2); (cv "f3", fun3)].
+
+Definition funTC23 : funTC := [(cv "f2", funFTyp fun2);
+                                (cv "f3", funFTyp fun3)].
+
+
+Lemma noDup_fun23 : noDup funEnv23.
+  econstructor.
+  simpl.
+  intuition.
+  inversion H0.
+  econstructor.
+  intuition.
+  econstructor.
+Defined.  
+  
+Lemma FEnvWT_fun23 : FEnvWT funEnv23.
+  unfold FEnvWT, FunWT, funEnv23, fun2, fun3.
+  intros.
+  unfold FEnvTyping in H.
+  unfold MatchEnvs in H.
+  unfold thicken in *.
+  inversion H; subst.  
+  destruct f.
+  simpl in *.
+  clear H1.
+  destruct (ModNat1.IdEqDec x (cv "f2")).
+  inversion e0; subst.
+  inversion H0; subst.
+  simpl in *.
+  econstructor.
+  instantiate (1:=PT[Nat]).
+  unfold IdFTyping.
+  unfold EnvrAssign.
+  simpl.
+  reflexivity.
+  econstructor.
+  econstructor.
+  econstructor.
+  econstructor.
+  destruct (ModNat1.IdEqDec x (cv "f3")).
+  inversion e0; subst.
+  inversion H0; subst.
+  econstructor.
+  econstructor.
+  econstructor.
+  inversion H0.
+Defined.  
+
+
+Definition exp8 : Exp := Call (cv "f3") (PS [exp7]).
+
+Lemma ExpTyping_exp8 : ExpTyping funTC23 nil exp8 Nat.
+repeat econstructor.
+Defined.
+
+Lemma FunWT_exp8 : FunWT (funEnv2funTC funEnv23)
+                         (FC nil (cst Nat (0%nat)) exp8).
+  repeat econstructor.
+Defined.  
+
+
+Definition test_top8 := TopLevel 100 nil funEnv23 
+                                   FEnvWT_fun23 noDup_fun23
+                                   (cst Nat (0%nat))
+                                   exp8 FunWT_exp8.
+
+Eval compute in test_top8.
+
+
+End CTest.
+
+  
