src/DEC2/ModNat1I1.v
@@ -1,0 +1,41 @@
+(* Paolo Torrini, 
+   Universite' Lille-1 - CRIStAL-CNRS
+*)
+(* example of concrete module *)
+
+Require Import AuxLibI1.
+Require Import TypSpecI1.
+Require Import ModTypI1.
+Require Import List.
+Require Import String.
+Require Import PeanoNat.
+Require Import Omega.
+
+
+Module ModNat1 <: ModTyp.
+
+  Definition Id := string.
+
+  Definition IdEqDec := string_dec.
+
+  Instance IdEq2 : DEq Id :=
+  {
+  dEq := IdEqDec
+  }.
+
+  Definition IdEq := IdEq2.
+  
+
+  Definition W := nat.
+
+  Definition BInit := 0.
+  
+  Instance WP2 : PState W :=
+  {  
+  b_init := BInit
+  }.              
+
+  Definition WP := WP2.
+  
+End ModNat1.
+
